chore: improve consistency documentation for hash table `insert` and `insertMany`

src/Std/Data/DHashMap/Internal/Defs.lean
@@ -407,14 +407,14 @@ variable {β : Type v}
   return r
 
 /-- Internal implementation detail of the hash map -/
-@[inline] def Const.insertManyUnit {ρ : Type w} [ForIn Id ρ α] [BEq α] [Hashable α]
+@[inline] def Const.insertManyIfNewUnit {ρ : Type w} [ForIn Id ρ α] [BEq α] [Hashable α]
     (m : Raw₀ α (fun _ => Unit)) (l : ρ) :
     { m' : Raw₀ α (fun _ => Unit) // ∀ (P : Raw₀ α (fun _ => Unit) → Prop),
-      (∀ {m'' a b}, P m'' → P (m''.insert a b)) → P m → P m' } := Id.run do
+      (∀ {m'' a b}, P m'' → P (m''.insertIfNew a b)) → P m → P m' } := Id.run do
   let mut r : { m' : Raw₀ α (fun _ => Unit) // ∀ (P : Raw₀ α (fun _ => Unit) → Prop),
-    (∀ {m'' a b}, P m'' → P (m''.insert a b)) → P m → P m' } := ⟨m, fun _ _ => id⟩
+    (∀ {m'' a b}, P m'' → P (m''.insertIfNew a b)) → P m → P m' } := ⟨m, fun _ _ => id⟩
   for a in l do
-    r := ⟨r.1.insert a (), fun _ h hm => h (r.2 _ h hm)⟩
+    r := ⟨r.1.insertIfNew a (), fun _ h hm => h (r.2 _ h hm)⟩
   return r
 
 end
