src/Std/Data/DHashMap/Raw.lean
@@ -58,7 +58,12 @@ instance : Inhabited (Raw α β) where
   default := ∅
 
 /--
-Inserts the given mapping into the map, replacing an existing mapping for the key if there is one.
+Inserts the given mapping into the map. If there is already a mapping for the given key, then both
+key and value will be replaced.
+
+Note: this replacement behavior is true for `HashMap`, `DHashMap`, `HashMap.Raw` and `DHashMap.Raw`.
+The `insert` function on `HashSet` and `HashSet.Raw` behaves differently: it will return the set
+unchanged if a matching key is already present.
 -/
 @[inline] def insert [BEq α] [Hashable α] (m : Raw α β) (a : α) (b : β a) : Raw α β :=
   if h : 0 < m.buckets.size then
@@ -373,6 +378,10 @@ instance : ForIn m (Raw α β) ((a : α) × β a) where
 /--
 Inserts multiple mappings into the hash map by iterating over the given collection and calling
 `insert`. If the same key appears multiple times, the last occurrence takes precedence.
+
+Note: this precedence behavior is true for `HashMap`, `DHashMap`, `HashMap.Raw` and `DHashMap.Raw`.
+The `insert` function on `HashSet` and `HashSet.Raw` behaves differently: it will prefer the first
+appearance.
 -/
 @[inline] def insertMany [BEq α] [Hashable α] {ρ : Type w} [ForIn Id ρ ((a : α) × β a)]
     (m : Raw α β) (l : ρ) : Raw α β :=
@@ -388,15 +397,16 @@ Inserts multiple mappings into the hash map by iterating over the given collecti
 
 /--
 Inserts multiple keys with the value `()` into the hash map by iterating over the given collection
-and calling `insert`. If the same key appears multiple times, the last occurrence takes precedence.
+and calling `insertIfNew`. If the same key appears multiple times, the first occurrence takes
+precedence.
 
 This is mainly useful to implement `HashSet.insertMany`, so if you are considering using this,
 `HashSet` or `HashSet.Raw` might be a better fit for you.
 -/
-@[inline] def Const.insertManyUnit [BEq α] [Hashable α] {ρ : Type w}
+@[inline] def Const.insertManyIfNewUnit [BEq α] [Hashable α] {ρ : Type w}
     [ForIn Id ρ α] (m : Raw α (fun _ => Unit)) (l : ρ) : Raw α (fun _ => Unit) :=
   if h : 0 < m.buckets.size then
-    (Raw₀.Const.insertManyUnit ⟨m, h⟩ l).1
+    (Raw₀.Const.insertManyIfNewUnit ⟨m, h⟩ l).1
   else m -- will never happen for well-formed inputs
 
 /-- Creates a hash map from a list of mappings. If the same key appears multiple times, the last
@@ -420,7 +430,7 @@ This is mainly useful to implement `HashSet.ofList`, so if you are considering u
 `HashSet` or `HashSet.Raw` might be a better fit for you. -/
 @[inline] def Const.unitOfList [BEq α] [Hashable α] (l : List α) :
     Raw α (fun _ => Unit) :=
-  Const.insertManyUnit ∅ l
+  Const.insertManyIfNewUnit ∅ l
 
 /-- Creates a hash map from an array of keys, associating the value `()` with each key.
 
@@ -428,7 +438,7 @@ This is mainly useful to implement `HashSet.ofArray`, so if you are considering 
 `HashSet` or `HashSet.Raw` might be a better fit for you. -/
 @[inline] def Const.unitOfArray [BEq α] [Hashable α] (l : Array α) :
     Raw α (fun _ => Unit) :=
-  Const.insertManyUnit ∅ l
+  Const.insertManyIfNewUnit ∅ l
 
 /--
 Returns the number of buckets in the internal representation of the hash map. This function may be
@@ -547,10 +557,10 @@ theorem WF.Const.insertMany {β : Type v} [BEq α] [Hashable α] {ρ : Type w} [
   simpa [Raw.Const.insertMany, h.size_buckets_pos] using
     (Raw₀.Const.insertMany ⟨m, h.size_buckets_pos⟩ l).2 _ WF.insert₀ h
 
-theorem WF.Const.insertManyUnit [BEq α] [Hashable α] {ρ : Type w} [ForIn Id ρ α]
-    {m : Raw α (fun _ => Unit)} {l : ρ} (h : m.WF) : (Const.insertManyUnit m l).WF := by
-  simpa [Raw.Const.insertManyUnit, h.size_buckets_pos] using
-    (Raw₀.Const.insertManyUnit ⟨m, h.size_buckets_pos⟩ l).2 _ WF.insert₀ h
+theorem WF.Const.insertManyIfNewUnit [BEq α] [Hashable α] {ρ : Type w} [ForIn Id ρ α]
+    {m : Raw α (fun _ => Unit)} {l : ρ} (h : m.WF) : (Const.insertManyIfNewUnit m l).WF := by
+  simpa [Raw.Const.insertManyIfNewUnit, h.size_buckets_pos] using
+    (Raw₀.Const.insertManyIfNewUnit ⟨m, h.size_buckets_pos⟩ l).2 _ WF.insertIfNew₀ h
 
 theorem WF.ofList [BEq α] [Hashable α] {l : List ((a : α) × β a)} :
     (ofList l : Raw α β).WF :=
@@ -562,7 +572,7 @@ theorem WF.Const.ofList {β : Type v} [BEq α] [Hashable α] {l : List (α × β
 
 theorem WF.Const.unitOfList [BEq α] [Hashable α] {l : List α} :
     (Const.unitOfList l : Raw α (fun _ => Unit)).WF :=
-  Const.insertManyUnit WF.empty
+  Const.insertManyIfNewUnit WF.empty
 
 end WF
 
